examples/C_Model_core.thy
@@ -1,0 +1,159 @@
+(******************************************************************************
+ * Language.C
+ * https://hackage.haskell.org/package/language-c
+ *
+ * Copyright (c) 1999-2017 Manuel M T Chakravarty
+ *                         Duncan Coutts
+ *                         Benedikt Huber
+ * Portions Copyright (c) 1989,1990 James A. Roskind
+ *
+ *  *  *  *  *  *  *  *  *  *  *  *  *  *  *  *  *  *  *  *  *  *  *  *  *  *
+ *
+ * Language.C.Comments
+ * https://hackage.haskell.org/package/language-c-comments
+ *
+ * Copyright (c) 2010-2014 Geoff Hulette
+ *
+ *  *  *  *  *  *  *  *  *  *  *  *  *  *  *  *  *  *  *  *  *  *  *  *  *  *
+ *
+ * Securify & Orca
+ *
+ * Copyright (c) 2016-2017 Nanyang Technological University, Singapore
+ *               2017-2018 Virginia Tech, USA
+ *
+ *  *  *  *  *  *  *  *  *  *  *  *  *  *  *  *  *  *  *  *  *  *  *  *  *  *
+ *
+ * All rights reserved.
+ *
+ * Redistribution and use in source and binary forms, with or without
+ * modification, are permitted provided that the following conditions are
+ * met:
+ *
+ *     * Redistributions of source code must retain the above copyright
+ *       notice, this list of conditions and the following disclaimer.
+ *
+ *     * Redistributions in binary form must reproduce the above
+ *       copyright notice, this list of conditions and the following
+ *       disclaimer in the documentation and/or other materials provided
+ *       with the distribution.
+ *
+ *     * Neither the name of the copyright holders nor the names of its
+ *       contributors may be used to endorse or promote products derived
+ *       from this software without specific prior written permission.
+ *
+ * THIS SOFTWARE IS PROVIDED BY THE COPYRIGHT HOLDERS AND CONTRIBUTORS
+ * "AS IS" AND ANY EXPRESS OR IMPLIED WARRANTIES, INCLUDING, BUT NOT
+ * LIMITED TO, THE IMPLIED WARRANTIES OF MERCHANTABILITY AND FITNESS FOR
+ * A PARTICULAR PURPOSE ARE DISCLAIMED. IN NO EVENT SHALL THE COPYRIGHT
+ * OWNER OR CONTRIBUTORS BE LIABLE FOR ANY DIRECT, INDIRECT, INCIDENTAL,
+ * SPECIAL, EXEMPLARY, OR CONSEQUENTIAL DAMAGES (INCLUDING, BUT NOT
+ * LIMITED TO, PROCUREMENT OF SUBSTITUTE GOODS OR SERVICES; LOSS OF USE,
+ * DATA, OR PROFITS; OR BUSINESS INTERRUPTION) HOWEVER CAUSED AND ON ANY
+ * THEORY OF LIABILITY, WHETHER IN CONTRACT, STRICT LIABILITY, OR TORT
+ * (INCLUDING NEGLIGENCE OR OTHERWISE) ARISING IN ANY WAY OUT OF THE USE
+ * OF THIS SOFTWARE, EVEN IF ADVISED OF THE POSSIBILITY OF SUCH DAMAGE.
+ ******************************************************************************)
+
+section \<open>Acknowledgements\<close>
+
+theory C_Model_core
+  imports "$HASKABELLE_HOME_USER/default/Prelude"
+          "../src/UML_Main"
+          "../src/compiler/Generator_dynamic_parallel"
+          C_Model_init
+begin
+
+subsection \<open>\<^file>\<open>$HASKABELLE_HOME/ex/language-c/AUTHORS.c2hs\<close>\<close>
+text \<open>
+  Manuel M T Chakravarty	<chak@cse.unsw.edu.au>
+  Duncan Coutts		<duncan@haskell.org>
+  
+  with contributions from (alphabetical order)
+  
+  Bertram Felgenhauer	<int-e@gmx.de>
+  Ian Lynagh		<igloo@earth.li>
+  André Pang		<ozone@algorithm.com.au>
+  Jens-Ulrik Petersen	<petersen@haskell.org>
+  Armin Sander		<armin@mindwalker.org>
+  Sean Seefried		<sseefried@cse.unsw.edu.au>
+  Udo Stenzel		<u.stenzel@web.de>
+  Axel Simon              <A.Simon@ukc.ac.uk>
+  Michael Weber		<michaelw@debian.org>
+  
+  Thanks for comments and suggestions to 
+  
+  Roman Leshchinskiy	<rl@cs.tu-berlin.de>
+  Jan Kort		<kort@science.uva.nl>
+  Seth Kurtzberg		<seth@cql.com>
+  Simon Marlow		<simonmar@microsoft.com>
+  Matthias Neubauer	<neubauer@informatik.uni-freiburg.de>
+  Sven Panne		<sven.panne@aedion.de>
+  Simon L. Peyton Jones	<simonpj@microsoft.com>
+  Volker Wysk		<post@volker-wysk.de>
+\<close>
+
+subsection \<open>\<^file>\<open>$HASKABELLE_HOME/ex/language-c/AUTHORS\<close>\<close>
+text \<open>
+  Benedikt Huber          <benedikt.huber@gmail.com>
+  Manuel M T Chakravarty  <chak@cse.unsw.edu.au>
+  Duncan Coutts           <duncan@haskell.org>
+  Bertram Felgenhauer     <int-e@gmx.de>
+  
+  with code contributions and patches from
+  
+  Iavor Diatchki          <iavor.diatchki@gmail.com>
+  Kevin Charter           <kcharter@gmail.com>
+  Aleksey Kliger
+  
+  This project originated from the C parser component of c2hs,
+  for many additional contributors see AUTHORS.c2hs.
+  
+  Special thanks for their great support, comments and suggestions to:
+  
+  Duncan Coutts           <duncan@haskell.org>
+  Iavor Diatchki          <iavor.diatchki@gmail.com>
+  Don Steward             <dons@galois.com>
+\<close>
+
+section \<open>Initialization of the generator\<close>
+
+declare [[syntax_ambiguity_warning = false]]
+
+generation_syntax [ deep
+                      (THEORY Meta_C_generated)
+                      (IMPORTS ["../src/UML_Main", "../src/compiler/Static", "../examples/C_Model_init"]
+                               "../src/compiler/Generator_dynamic_parallel")
+                      SECTION
+                      SORRY
+                      [ in self ]
+                      (output_directory "../doc")
+                  , shallow SORRY ]
+
+section \<open>Type definition\<close>
+
+End!
+
+text \<open> \<^file>\<open>$HASKABELLE_HOME/ex/language-c/src/Language/C/Data/Name.hs\<close>
+       \<^file>\<open>$HASKABELLE_HOME/ex/language-c/src/Language/C/Data/Position.hs\<close>
+       \<^file>\<open>$HASKABELLE_HOME/ex/language-c/src/Language/C/Data/Node.hs\<close>
+       \<^file>\<open>$HASKABELLE_HOME/ex/language-c/src/Language/C/Data/Ident.hs\<close>
+       \<^file>\<open>$HASKABELLE_HOME/ex/language-c/src/Language/C/Syntax/Ops.hs\<close>
+       \<^file>\<open>$HASKABELLE_HOME/ex/language-c/src/Language/C/Syntax/Constants.hs\<close> \<close>
+
+Haskell_file datatype_old_atomic try_import only_types concat_modules
+             base_path "$HASKABELLE_HOME/ex/language-c/src"
+             [Prelude \<rightharpoonup> C_Model_init, Int, String, Option \<rightharpoonup> C_Model_init]
+             (**)
+             "$HASKABELLE_HOME/ex/language-c/src/Language/C/Syntax/AST.hs"
+
+text \<open>@{typ CTranslUnit}\<close>
+
+datatype CommentFormat = SingleLine | MultiLine
+datatype Comment = Comment Position string CommentFormat
+
+section \<open>Garbage Collection of Notations\<close>
+
+hide_type (open) int
+hide_type (open) string
+
+end
